First pass at refactoring pagedb.dfy. This verifies still.

verified/pagedb.dfy
@@ -68,17 +68,21 @@ predicate validPageDbEntryTyped(d: PageDb, n: PageNr)
     requires n in d && d[n].PageDbEntryTyped?
 {
     var e := d[n].entry;
-    (wellFormedPageDbEntry(d, e) || stoppedAddrspace(d, n)) &&
+    // (wellFormedPageDbEntry(d, e) || stoppedAddrspace(d, n)) &&
+    closedRefsPageDbEntry(d, e) &&
     pageDbEntryWellTypedAddrspace(d, n)
     //|| stoppedAddrspace(d, n)
 }
 
+predicate isAddrspace(d: PageDb, n: PageNr)
+    { n in d && d[n].PageDbEntryTyped? && d[n].entry.Addrspace? }
+
+// The addrspace of the thing pointed to by n is stopped
 predicate stoppedAddrspace(d: PageDb, n: PageNr)
     requires n in d && d[n].PageDbEntryTyped?
 {
     var a := d[n].addrspace;
-    a in d && d[a].PageDbEntryTyped? && d[a].entry.Addrspace? &&
-        d[a].entry.state == StoppedState
+    isAddrspace(d, a) && d[a].entry.state == StoppedState
 }
 
 
@@ -89,9 +93,7 @@ predicate pageDbEntryWellTypedAddrspace(d: PageDb, n: PageNr)
 {
     var entry := d[n].entry;
     var addrspace := d[n].addrspace;
-    addrspace in d
-    && d[addrspace].PageDbEntryTyped?
-    && d[addrspace].entry.Addrspace?
+    isAddrspace(d, addrspace)
     // Type-specific requirements
     && ( (entry.Addrspace? && addrspaceOkAddrspace(d, n, addrspace))
        || (entry.L1PTable? && (stoppedAddrspace(d, n) || addrspaceOkL1PTable(d, n, addrspace)))
@@ -109,12 +111,23 @@ predicate addrspaceOkAddrspace(d: PageDb, n: PageNr, a: PageNr)
         n == a
         && addrspaceL1Unique(d, a)
         && addrspace.refcount == |addrspaceRefs(d, a)|
+
+        // Not needed when stopped
         && (stoppedAddrspace(d, n) ||  (
             d[addrspace.l1ptnr].PageDbEntryTyped? &&
             d[addrspace.l1ptnr].entry.L1PTable? &&
             d[addrspace.l1ptnr].addrspace == n
         ))
-        // TODO CHECK L1PTPAGE UNIQUENESS HERE
+}
+
+predicate addrspaceL1Unique(d: PageDb, n: PageNr)
+    requires n in d && d[n].PageDbEntryTyped? && d[n].entry.Addrspace?
+{
+    var a := d[n].entry;
+    a.l1ptnr in d &&
+    forall p :: p in d && p != a.l1ptnr &&
+        d[p].PageDbEntryTyped? && d[p].addrspace == n ==>
+        !d[p].entry.L1PTable?
 }
 
 predicate addrspaceOkL1PTable(d: PageDb, n: PageNr, a: PageNr)
@@ -123,49 +136,9 @@ predicate addrspaceOkL1PTable(d: PageDb, n: PageNr, a: PageNr)
 {
     var e := d[n];
     var l1pt := e.entry.l1pt;
-    // var addrspace := d[a].entry;
     // addrspace.l1ptnr == n &&
     forall pte :: pte in l1pt && pte.Just? ==> ( var pteE := fromJust(pte);
-        pteE in d && d[pteE].PageDbEntryTyped? && d[pteE].addrspace == a)
-}
-
-predicate addrspaceOkL2PTable(d: PageDb, n: PageNr, a: PageNr)
-    requires n in d && d[n].PageDbEntryTyped? && d[n].entry.L2PTable?
-    requires a in d && d[a].PageDbEntryTyped? && d[a].entry.Addrspace?
-{
-    var e := d[n];
-    var l2pt := e.entry.l2pt;
-    forall pte :: pte in l2pt && pte.SecureMapping? ==> (
-        var ptePg := pte.page;
-        ptePg in d && d[ptePg].PageDbEntryTyped? && d[ptePg].addrspace == a)
-}
-
-predicate wellFormedPageDbEntry(d: PageDb, e: PageDbEntryTyped)
-{
-    (e.Addrspace? &&  validAddrspace(d, e))
-    || (e.L1PTable? && validL1PTable(d, e))
-    || (e.L2PTable? && validL2PTable(d, e))
-    || (e.Dispatcher? )
-    || (e.DataPage? )
-}
-
-// Free pages and non-addrspace entries should have a refcount of 0
-predicate pageDbEntryValidRefs(d: PageDb, n: PageNr)
-    requires n in d
-{
-    var e := d[n];
-    (e.PageDbEntryTyped? && e.entry.Addrspace?) ||
-        forall m : PageNr :: validPageNr(m) ==>
-            |addrspaceRefs(d, n)| == 0
-}
-
-predicate validL1PTable(d: PageDb, e: PageDbEntryTyped)
-    requires e.L1PTable?
-    // requires var a := d[n].addrspace; a in d && d[a].PageDbEntryTyped? && d[a].entry.Addrspace?
-{
-    var l1pt := e.l1pt;
-    // it's the right length (all page tables are this length)
-    |l1pt| == NR_L1PTES()
+        pteE in d && d[pteE].PageDbEntryTyped? && d[pteE].addrspace == a )
     // each non-zero entry is a valid L2PT belonging to this address space
     && forall pte :: pte in l1pt && pte.Just? ==> validL1PTE(d, fromJust(pte))
     // no L2PT is referenced twice
@@ -180,11 +153,16 @@ predicate validL1PTE(d: PageDb, pte: PageNr)
         && d[pte].entry.L2PTable?
 }
 
-predicate validL2PTable(d: PageDb, e: PageDbEntryTyped)
-    requires e.L2PTable?
+predicate addrspaceOkL2PTable(d: PageDb, n: PageNr, a: PageNr)
+    requires n in d && d[n].PageDbEntryTyped? && d[n].entry.L2PTable?
+    requires a in d && d[a].PageDbEntryTyped? && d[a].entry.Addrspace?
 {
-    var l2pt := e.l2pt;
-    |l2pt| == NR_L2PTES()
+    var e := d[n];
+    var l2pt := e.entry.l2pt;
+    forall pte :: pte in l2pt && pte.SecureMapping? ==> (
+        var ptePg := pte.page;
+        ptePg in d && d[ptePg].PageDbEntryTyped? && d[ptePg].addrspace == a)
+    // Not needed when addrspace is stopped 
     // each secure entry is a valid data page belonging to this address space
     && forall pte :: pte in l2pt && pte.SecureMapping?
         ==> validL2PTE(d, pte.page)
@@ -197,31 +175,45 @@ predicate validL2PTE(d: PageDb, pte: PageNr)
         && d[pte].entry.DataPage?
 }
 
-predicate validAddrspacePage(d: PageDb, n: PageNr)
+
+// Free pages and non-addrspace entries should have a refcount of 0
+predicate pageDbEntryValidRefs(d: PageDb, n: PageNr)
+    requires n in d
 {
-    n in d && d[n].PageDbEntryTyped? && d[n].entry.Addrspace? &&
-        validAddrspace(d, d[n].entry)
-}
-   
-predicate validAddrspace(d: PageDb, a: PageDbEntryTyped)
-    requires a.Addrspace?
-{
-        a.state == StoppedState || 
-        (validPageNr(a.l1ptnr)
-        && a.l1ptnr in d
-        && d[a.l1ptnr].PageDbEntryTyped?
-        && d[a.l1ptnr].entry.L1PTable?)
+    var e := d[n];
+    (e.PageDbEntryTyped? && e.entry.Addrspace?) ||
+        forall m : PageNr :: validPageNr(m) ==>
+            |addrspaceRefs(d, n)| == 0
 }
 
-predicate addrspaceL1Unique(d: PageDb, n: PageNr)
-    requires n in d && d[n].PageDbEntryTyped? && d[n].entry.Addrspace?
+predicate closedRefsPageDbEntry(d: PageDb, e: PageDbEntryTyped)
 {
-    var a := d[n].entry;
-    a.l1ptnr in d &&
-    forall p :: p in d && p != a.l1ptnr &&
-        d[p].PageDbEntryTyped? && d[p].addrspace == n ==>
-        !d[p].entry.L1PTable?
+    (e.Addrspace? && e.l1ptnr in d )
+    || (e.L1PTable? && closedRefsL1PTable(d, e))
+    || (e.L2PTable? && closedRefsL2PTable(d, e))
+    || (e.Dispatcher? )
+    || (e.DataPage? )
 }
+
+predicate closedRefsL1PTable(d: PageDb, e: PageDbEntryTyped)
+    requires e.L1PTable?
+{
+    var l1pt := e.l1pt;
+    |l1pt| == NR_L1PTES()
+    && forall pte :: pte in l1pt && pte.Just? ==> fromJust(pte) in d
+}
+
+predicate closedRefsL2PTable(d: PageDb, e: PageDbEntryTyped)
+    requires e.L2PTable?
+{
+    var l2pt := e.l2pt;
+    |l2pt| == NR_L2PTES()
+    && forall pte :: pte in l2pt ==> (match pte
+        case SecureMapping(p, w, e) => p in d
+        case InsecureMapping(p) => p in d
+        case NoMapping => true)
+}
+
 
 
 // returns the number of references to an addrspace page with the given index
